Types/Stores.v
@@ -1,12 +1,17 @@
+Require Export Base.
 Require Import Types.Maps.
 Require Import Language.Statements.
 
 Definition abstract_store := total_map avalue.
 Definition store := total_map cvalue.
 
+Instance abstract_store_inhabited : Inhabited abstract_store := λ _, VTop.
+Instance concrete_store_inhabited : Inhabited store := λ _, VNat 0.
+
 Definition abstract_update (s : abstract_store) (x : string) (v : avalue) :
   abstract_store := t_update s x v.
 
 Definition concrete_update (s : store) (x : string) (v : cvalue) :
   store := t_update s x v.
+
 
